Fixed up to DM_Inference.thy to use string literals

inference-tool/src/main/scala/inference/FrontEnd.scala
@@ -21,9 +21,9 @@ object FrontEnd {
     println("Hello inference!")
     val inferred = (Inference.learn(log, (SelectionStrategies.naive_score _).curried, (Inference.null_generator _).curried, (Inference.null_modifier _).curried))
 
-    // println("The inferred machine is deterministic?"+Inference.nondeterminism(Inference.toiEFSM(inferred)))
+    println("The inferred machine is "+(if (Inference.nondeterminism(Inference.toiEFSM(inferred))) "non" else "")+"deterministic")
 
-    val pw = new PrintWriter(new File("dotfiles/drinks.dot" ))
+    val pw = new PrintWriter(new File("dotfiles/vend1.dot" ))
     pw.write(EFSM_Dot.efsm2dot(inferred))
     pw.close
 
