formal/EFSM.thy
@@ -13,8 +13,10 @@ begin
 type_synonym event = "(label \<times> inputs)"
 type_synonym trace = "event list"
 type_synonym observation = "outputs list"
-
 type_synonym transition_matrix = "((nat \<times> nat) \<times> transition) fset"
+
+abbreviation Str :: "string \<Rightarrow> value" where
+  "Str s \<equiv> value.Str (String.implode s)"
 
 primrec input2state :: "value list \<Rightarrow> nat \<Rightarrow> datastate" where
   "input2state [] _ = <>" |
