formal/inference/DM_Inference.thy
@@ -1,11 +1,18 @@
 theory DM_Inference
-imports Inference SelectionStrategies "../examples/Drinks_Machine_2" EFSM_Dot
+  imports Inference SelectionStrategies "../examples/Drinks_Machine_2" EFSM_Dot
 begin
 
 declare One_nat_def[simp del]
 
-lemma "max coin vend = vend"
-  by (simp add: max_def coin_def vend_def less_eq_transition_ext_def less_transition_ext_def)
+lemma str_coin_lt_str_vend: "STR ''coin'' < STR ''vend''"
+proof-
+  have explode_coin: "literal.explode STR ''coin'' = ''coin''"
+    using Literal.rep_eq zero_literal.rep_eq by auto
+  have explode_vend: "literal.explode STR ''vend'' = ''vend''"
+    using Literal.rep_eq zero_literal.rep_eq by auto
+  show ?thesis
+    by (simp add: String.less_literal_def explode_coin explode_vend)
+qed
 
 definition drinks2 :: iEFSM where
   "drinks2 = {|(0, (0, 1), select),
@@ -133,6 +140,7 @@ lemma vend_fail_subsumes_vend_nothing: "subsumes select_posterior vend_fail vend
      apply (simp add: guard_vend_nothing medial_vend_fail)
      apply (simp add: select_posterior_def)
      apply auto[1]  
+     apply (simp add: transitions)
     apply (simp add: transitions)
    apply (simp add: medial_vend_nothing )
    apply (simp add: vend_nothing_posterior )
@@ -162,7 +170,7 @@ lemma vend_nothing_exits_1[simp]: "exits_state drinks2 vend_nothing 1"
 
 definition coin50 :: "transition" where
 "coin50 \<equiv> \<lparr>
-        Label = ''coin'',
+        Label = STR ''coin'',
         Arity = 1,
         Guard = [(gexp.Eq (V (I 1)) (L (Num 50)))],
         Outputs = [Plus (V (R 2)) (V (I 1))],
@@ -275,15 +283,15 @@ proof-
 qed
 
 lemma coin_lt_vend_nothing: "coin < vend_nothing"
-  by (simp add: transitions less_transition_ext_def)
+  by (simp add: transitions less_transition_ext_def str_coin_lt_str_vend)
 
 lemma tm_drinks2: "tm drinks2 = Drinks_Machine_2.drinks2"
   by (simp add: tm_def drinks2_def Drinks_Machine_2.drinks2_def)
 
-lemma step_merge_1_2_select: " length b = 1 \<Longrightarrow> step (tm merged_1_2) 0 Map.empty ''select'' b = Some (select, 1, [], <R 1 := hd b, R 2 := Num 0>)"
+lemma step_merge_1_2_select: " length b = 1 \<Longrightarrow> step (tm merged_1_2) 0 Map.empty (STR ''select'') b = Some (select, 1, [], <R 1 := hd b, R 2 := Num 0>)"
 proof-
   assume premise: "length b = 1"
-  have possible_steps: "possible_steps (tm merged_1_2) 0 Map.empty ''select'' b = {|(1, select)|}"
+  have possible_steps: "possible_steps (tm merged_1_2) 0 Map.empty (STR ''select'') b = {|(1, select)|}"
     apply (simp add: possible_steps_def ffilter_def tm_def merged_1_2_def fimage_def fset_both_sides Abs_fset_inverse)
     apply (simp add: Set.filter_def)
     apply safe
@@ -298,10 +306,10 @@ proof-
 qed
 
 lemma step_merge_1_2_vend_nothing: "\<nexists>n. ra (R 2) = Some (Num n) \<Longrightarrow>
-       step (tm merged_1_2) 1 ra ''vend'' [] = Some (vend_nothing, 1, [], ra)"
+       step (tm merged_1_2) 1 ra (STR ''vend'') [] = Some (vend_nothing, 1, [], ra)"
 proof-
   assume premise: "\<nexists>n. ra (R 2) = Some (Num n)"
-  have possible_steps: "possible_steps (tm merged_1_2) 1 ra ''vend'' [] = {|(1, vend_nothing)|}"
+  have possible_steps: "possible_steps (tm merged_1_2) 1 ra (STR ''vend'') [] = {|(1, vend_nothing)|}"
     apply (case_tac "ra (R 2)")
     apply (simp add: possible_steps_def ffilter_def tm_def merged_1_2_def fimage_def)
     apply (simp add: fset_both_sides Abs_fset_inverse)
@@ -322,7 +330,7 @@ proof-
     by simp
 qed
 
-lemma possible_steps_merge_coin: "length i = 1 \<Longrightarrow> possible_steps (tm merged_1_2) 1 r ''coin'' i = {|(1, coin)|}"
+lemma possible_steps_merge_coin: "length i = 1 \<Longrightarrow> possible_steps (tm merged_1_2) 1 r (STR ''coin'') i = {|(1, coin)|}"
   apply (simp add: possible_steps_def ffilter_def tm_def merged_1_2_def fimage_def)
   apply (simp add: fset_both_sides Abs_fset_inverse)
   apply (simp add: Set.filter_def transitions)
@@ -330,12 +338,12 @@ lemma possible_steps_merge_coin: "length i = 1 \<Longrightarrow> possible_steps 
 
 lemma step_merge_1_2_vend: "d' (R 2) = Some (Num x1) \<Longrightarrow>
        x1 < 100 \<Longrightarrow>
-       step (tm merged_1_2) 1 d' ''vend'' [] = None"
+       step (tm merged_1_2) 1 d' (STR ''vend'') [] = None"
 
 proof-
   assume premise1: "d' (R 2) = Some (Num x1)"
   assume premise2: "x1 < 100"
-  have possible_steps: "possible_steps (tm merged_1_2) 1 d' ''vend'' [] = {|(1, vend_nothing), (1, vend_fail)|}"
+  have possible_steps: "possible_steps (tm merged_1_2) 1 d' (STR ''vend'') [] = {|(1, vend_nothing), (1, vend_fail)|}"
     apply (simp add: possible_steps_def ffilter_def tm_def merged_1_2_def fimage_def)
     apply (simp add: fset_both_sides Abs_fset_inverse)
     apply (simp add: Set.filter_def)
@@ -349,11 +357,11 @@ proof-
     by (simp add: transitions fis_singleton_def is_singleton_def)
 qed
 
-lemma step_merge_1_2_vend_2: "d' (R 2) = Some (Num n) \<Longrightarrow> n \<ge> 100 \<Longrightarrow> step (tm merged_1_2) 1 d' ''vend'' [] = None"
+lemma step_merge_1_2_vend_2: "d' (R 2) = Some (Num n) \<Longrightarrow> n \<ge> 100 \<Longrightarrow> step (tm merged_1_2) 1 d' (STR ''vend'') [] = None"
 proof-
   assume premise1: "d' (R 2) = Some (Num n)"
   assume premise2: "n \<ge> 100"
-  have possible_steps: "possible_steps (tm merged_1_2) 1 d' ''vend'' [] = {|(1, vend_nothing), (3, vend)|}"
+  have possible_steps: "possible_steps (tm merged_1_2) 1 d' (STR ''vend'') [] = {|(1, vend_nothing), (3, vend)|}"
     apply (simp add: possible_steps_def ffilter_def tm_def merged_1_2_def fimage_def)
     apply (simp add: fset_both_sides Abs_fset_inverse)
     apply (simp add: Set.filter_def)
@@ -390,7 +398,7 @@ next
     apply clarify
     apply simp
 
-    apply (case_tac "aa = ''vend'' \<and> b = []")
+    apply (case_tac "aa = STR ''vend'' \<and> b = []")
      apply simp
      apply (rule accepts.cases)
        apply simp
@@ -407,7 +415,7 @@ next
       defer
       apply (simp add: step_merge_1_2_vend_nothing vend_nothing_posterior)
 
-     apply (case_tac "aa = ''coin'' \<and> length b = 1")
+     apply (case_tac "aa = STR ''coin'' \<and> length b = 1")
       apply (rule accepts.cases)
         apply simp
        apply simp
@@ -452,7 +460,7 @@ next
 
       apply simp
      apply clarify
-     apply (case_tac "aa = ''select'' \<and> length ba = 1")
+     apply (case_tac "aa = STR ''select'' \<and> length ba = 1")
       apply (simp add: anterior_context_def step_merge_1_2_select select_posterior)
       apply (simp add: accepts_trace_def)
       apply (rule accepts.cases)
@@ -470,7 +478,9 @@ next
 qed
 
 lemma directly_subsumes_vend_fail_vend_nothing: "directly_subsumes (tm DM_Inference.drinks2) (tm merged_1_2) 1 vend_fail vend_nothing"
-  by (simp add: tm_drinks2 directly_subsumes_def directly_subsumes_aux vend_fail_subsumes_vend_nothing)
+  apply (simp add: tm_drinks2 directly_subsumes_def directly_subsumes_aux vend_fail_subsumes_vend_nothing)
+  using vend_fail_subsumes_vend_nothing
+  by auto
 
 definition two_coins :: iEFSM where
   "two_coins = {|(1, (1, 1), vend_fail), (0, (0, 1), select), (2, (1, 1), coin), (3, (1, 1), coin), (5, (1, 3), vend)|}"
@@ -489,41 +499,8 @@ proof-
 qed
 
 lemma merge_vend_nothing_vend: "merge_transitions DM_Inference.drinks2 merged_1_3 1 2 1 1 1 vend_nothing 1 vend 5 null_generator null_modifier True = None"
-proof-
-  have accepts_and_gets_us_to: " accepts_trace Drinks_Machine_2.drinks2 [(''select'', [Str ''coke'']), (''coin'', [Num 50])] \<and>
-    gets_us_to 2 Drinks_Machine_2.drinks2 0 Map.empty [(''select'', [Str ''coke'']), (''coin'', [Num 50])]"
-    apply standard
-     apply (simp add: accepts_trace_def)
-     apply (rule accepts.step)
-      apply simp
-      apply (simp add: step_def possible_steps_0)
-     apply (rule accepts.step)
-      apply (simp add: step_def possible_steps_1)
-     apply (rule accepts.base)
-    apply (rule gets_us_to.step_some)
-     apply (simp add: step_def possible_steps_0)
-    apply (rule gets_us_to.step_some)
-     apply (simp add: step_def possible_steps_1)
-    by (simp add: gets_us_to.base)
-  show ?thesis
   apply (simp add: merge_transitions_def easy_merge_def tm_drinks2 null_generator_def null_modifier_def)
-  apply (simp add: directly_subsumes_def)
-  apply standard
-     apply (rule_tac x="[(''select'', [Str ''coke'']), (''coin'', [Num 50])]" in exI)
-     apply (simp add: accepts_and_gets_us_to no_subsumption_vend_nothing_vend)
-    apply standard
-     apply (simp add: no_subsumption_vend_vend_nothing)
-    apply (rule_tac x="[(''select'', [Str ''coke''])]" in exI)
-    apply standard
-     apply (simp add: accepts_trace_def)
-     apply (rule accepts.step)
-      apply simp
-      apply (simp add: step_def possible_steps_0)
-     apply (rule accepts.base)
-    apply (rule gets_us_to.step_some)
-     apply (simp add: step_def possible_steps_0)
-    by (simp add: gets_us_to.base)
-qed
+  by (simp add: directly_subsumes_def no_subsumption_vend_nothing_vend no_subsumption_vend_vend_nothing)
 
 lemma nondeterministic_pairs_two_coins: "nondeterministic_pairs two_coins = {|
       (1, (1, 1),(coin,3),coin,2),
@@ -565,7 +542,7 @@ proof-
 qed
 
 lemma coin_lt_vend_fail: "coin < vend_fail"
-  by (simp add: transitions less_transition_ext_def)
+  by (simp add: transitions less_transition_ext_def str_coin_lt_str_vend)
 
 lemma subsumes_coin_coin: "subsumes c coin coin"
   apply (simp add: subsumes_def)
@@ -580,31 +557,31 @@ proof-
     apply (simp add: transitions)
     by auto
   have state_nondeterminism_1: "state_nondeterminism 1 {|(1, coin, 3), (1, vend_fail, 1), (3, vend, 5)|} = {|(1, (3, 1),
-    (\<lparr>Label = ''vend'', Arity = 0, Guard = [Ge (V (R 2)) (L (Num 100))], Outputs = [V (R 1)], Updates = [(R 1, V (R 1)), (R 2, V (R 2))]\<rparr>, 5),
-    \<lparr>Label = ''vend'', Arity = 0, Guard = [GExp.Lt (V (R 2)) (L (Num 100))], Outputs = [], Updates = [(R 1, V (R 1)), (R 2, V (R 2))]\<rparr>, 1),
+    (\<lparr>Label = STR ''vend'', Arity = 0, Guard = [Ge (V (R 2)) (L (Num 100))], Outputs = [V (R 1)], Updates = [(R 1, V (R 1)), (R 2, V (R 2))]\<rparr>, 5),
+    \<lparr>Label = STR ''vend'', Arity = 0, Guard = [GExp.Lt (V (R 2)) (L (Num 100))], Outputs = [], Updates = [(R 1, V (R 1)), (R 2, V (R 2))]\<rparr>, 1),
    (1, (3, 1),
-    (\<lparr>Label = ''vend'', Arity = 0, Guard = [Ge (V (R 2)) (L (Num 100))], Outputs = [V (R 1)], Updates = [(R 1, V (R 1)), (R 2, V (R 2))]\<rparr>, 5),
-    \<lparr>Label = ''coin'', Arity = 1, Guard = [], Outputs = [Plus (V (R 2)) (V (I 1))],
+    (\<lparr>Label = STR ''vend'', Arity = 0, Guard = [Ge (V (R 2)) (L (Num 100))], Outputs = [V (R 1)], Updates = [(R 1, V (R 1)), (R 2, V (R 2))]\<rparr>, 5),
+    \<lparr>Label = STR ''coin'', Arity = 1, Guard = [], Outputs = [Plus (V (R 2)) (V (I 1))],
        Updates = [(R 1, V (R 1)), (R 2, Plus (V (R 2)) (V (I 1)))]\<rparr>,
     3),
    (1, (1, 3),
-    (\<lparr>Label = ''vend'', Arity = 0, Guard = [GExp.Lt (V (R 2)) (L (Num 100))], Outputs = [], Updates = [(R 1, V (R 1)), (R 2, V (R 2))]\<rparr>, 1),
-    \<lparr>Label = ''vend'', Arity = 0, Guard = [Ge (V (R 2)) (L (Num 100))], Outputs = [V (R 1)], Updates = [(R 1, V (R 1)), (R 2, V (R 2))]\<rparr>, 5),
+    (\<lparr>Label = STR ''vend'', Arity = 0, Guard = [GExp.Lt (V (R 2)) (L (Num 100))], Outputs = [], Updates = [(R 1, V (R 1)), (R 2, V (R 2))]\<rparr>, 1),
+    \<lparr>Label = STR ''vend'', Arity = 0, Guard = [Ge (V (R 2)) (L (Num 100))], Outputs = [V (R 1)], Updates = [(R 1, V (R 1)), (R 2, V (R 2))]\<rparr>, 5),
    (1, (1, 1),
-    (\<lparr>Label = ''vend'', Arity = 0, Guard = [GExp.Lt (V (R 2)) (L (Num 100))], Outputs = [], Updates = [(R 1, V (R 1)), (R 2, V (R 2))]\<rparr>, 1),
-    \<lparr>Label = ''coin'', Arity = 1, Guard = [], Outputs = [Plus (V (R 2)) (V (I 1))],
+    (\<lparr>Label = STR ''vend'', Arity = 0, Guard = [GExp.Lt (V (R 2)) (L (Num 100))], Outputs = [], Updates = [(R 1, V (R 1)), (R 2, V (R 2))]\<rparr>, 1),
+    \<lparr>Label = STR ''coin'', Arity = 1, Guard = [], Outputs = [Plus (V (R 2)) (V (I 1))],
        Updates = [(R 1, V (R 1)), (R 2, Plus (V (R 2)) (V (I 1)))]\<rparr>,
     3),
    (1, (1, 3),
-    (\<lparr>Label = ''coin'', Arity = 1, Guard = [], Outputs = [Plus (V (R 2)) (V (I 1))],
+    (\<lparr>Label = STR ''coin'', Arity = 1, Guard = [], Outputs = [Plus (V (R 2)) (V (I 1))],
         Updates = [(R 1, V (R 1)), (R 2, Plus (V (R 2)) (V (I 1)))]\<rparr>,
      3),
-    \<lparr>Label = ''vend'', Arity = 0, Guard = [Ge (V (R 2)) (L (Num 100))], Outputs = [V (R 1)], Updates = [(R 1, V (R 1)), (R 2, V (R 2))]\<rparr>, 5),
+    \<lparr>Label = STR ''vend'', Arity = 0, Guard = [Ge (V (R 2)) (L (Num 100))], Outputs = [V (R 1)], Updates = [(R 1, V (R 1)), (R 2, V (R 2))]\<rparr>, 5),
    (1, (1, 1),
-    (\<lparr>Label = ''coin'', Arity = 1, Guard = [], Outputs = [Plus (V (R 2)) (V (I 1))],
+    (\<lparr>Label = STR ''coin'', Arity = 1, Guard = [], Outputs = [Plus (V (R 2)) (V (I 1))],
         Updates = [(R 1, V (R 1)), (R 2, Plus (V (R 2)) (V (I 1)))]\<rparr>,
      3),
-    \<lparr>Label = ''vend'', Arity = 0, Guard = [GExp.Lt (V (R 2)) (L (Num 100))], Outputs = [], Updates = [(R 1, V (R 1)), (R 2, V (R 2))]\<rparr>, 1)|}"
+    \<lparr>Label = STR ''vend'', Arity = 0, Guard = [GExp.Lt (V (R 2)) (L (Num 100))], Outputs = [], Updates = [(R 1, V (R 1)), (R 2, V (R 2))]\<rparr>, 1)|}"
     by eval
   show ?thesis
     apply (simp add: nondeterministic_pairs_def fimage_def S_def basically_drinks_def outgoing_transitions_def state_nondeterminism_1)
@@ -632,7 +609,7 @@ proof-
     by (simp add: score sorted_list_of_fset_def)
 qed
 
-lemma possible_steps_select_dm_2:  "possible_steps (tm DM_Inference.drinks2) 0 Map.empty ''select'' [Str ''coke''] = {|(1, select)|}"
+lemma possible_steps_select_dm_2:  "possible_steps (tm DM_Inference.drinks2) 0 Map.empty (STR ''select'') [Str ''coke''] = {|(1, select)|}"
   by eval
 
 lemma consistent_posterior_vend_nothing: "consistent c \<Longrightarrow> consistent (posterior c vend_nothing)"
@@ -714,37 +691,34 @@ lemma inconsistent_posterior_vend_fail: "\<not> consistent c \<Longrightarrow> \
 
 lemma vend_nothing_subsumes_vend_fail: "subsumes c vend_nothing vend_fail"
   apply (simp add: subsumes_def)
-  apply (standard, simp add: transitions)+
-   apply clarify
-   apply (case_tac "r = V (R 2)")
-    apply simp
-    apply clarify
-    apply (case_tac "ValueLt (Some i) (Some (Num 100))")
-     apply simp
-    apply simp
-    apply (case_tac "cval (c (V (R 2))) i")
-     apply simp
-    apply simp
-   apply simp
-   apply clarify
-   apply (case_tac "cval (c r) i")
-    apply simp
-   apply simp
-  apply standard
-   apply (simp add: transitions)
-  apply standard
-   defer
+  apply safe
+         apply (simp add: transitions)+
+      apply (case_tac "r = V (R 2)")
+       apply simp
+       apply clarify
+       apply (case_tac "ValueLt (Some i) (Some (Num 100))")
+        apply simp
+       apply simp
+       apply (case_tac "cval (c (V (R 2))) i")
+        apply simp
+       apply simp
+      apply simp
+      apply (case_tac "cval (c r) i")
+       apply simp
+      apply simp
+     apply (simp add: transitions)
+    apply (simp add: transitions)
    apply (case_tac "consistent c")
-    apply (simp add: consistent_posterior_vend_nothing)
-   apply (simp add: inconsistent_posterior_vend_fail)
-
-  apply clarify
-  apply (case_tac "consistent (\<lambda>r. and (if r = V (R 2) then snd (V (R 2), cexp.Lt (Num 100)) else cexp.Bc True) (c r))")
-  apply (simp add: posterior_def vend_nothing_def remove_input_constraints_def vend_fail_def)
-   apply (case_tac "ValueLt (Some i) (Some (Num 100))")
-    apply auto[1]
-   apply auto[1]
-  by (simp add: posterior_def vend_nothing_def remove_input_constraints_def vend_fail_def)
+    apply (simp add: transitions posterior_def)
+    apply (case_tac "consistent (\<lambda>r. and (if r = V (R 2) then snd (V (R 2), cexp.Lt (Num 100)) else cexp.Bc True) (c r))")
+     apply (simp add: remove_input_constraints_def)
+     apply (case_tac "ValueLt (Some i) (Some (Num 100))")
+      apply auto[1]
+     apply auto[1]
+    apply simp
+   apply (simp add: transitions posterior_def)
+   apply (simp add: inconsistent_c)
+  using consistent_posterior_vend_nothing inconsistent_posterior_vend_fail by blast
 
 lemma directly_subsumes_vend_nothing_vend_fail: "directly_subsumes (tm DM_Inference.drinks2) (tm merged_1_2) 2 vend_nothing vend_fail"
   by (simp add: directly_subsumes_def vend_nothing_subsumes_vend_fail)
@@ -806,7 +780,7 @@ definition "merged_1_3_2 = {|(5, (1, 1),
 lemma merge_1_3_2: "merge_states 3 1 merged_wrong_vends = merged_1_3_2 \<and> merge_states 1 3 merged_wrong_vends = merged_1_3_2"
   by eval
 
-lemma possible_steps_coin_dm_2: "possible_steps (tm drinks2) 1 r ''coin'' [Num n] = {|(2, coin)|}"
+lemma possible_steps_coin_dm_2: "possible_steps (tm drinks2) 1 r (STR ''coin'') [Num n] = {|(2, coin)|}"
     apply (simp add: possible_steps_def drinks2_def ffilter_def fimage_def fset_both_sides Abs_fset_inverse tm_def)
     apply (simp add: Set.filter_def)
     apply safe
@@ -814,8 +788,9 @@ lemma possible_steps_coin_dm_2: "possible_steps (tm drinks2) 1 r ''coin'' [Num n
   by force
 
 lemma no_direct_subsumption_vend_nothing_vend: "\<not> directly_subsumes (tm DM_Inference.drinks2) (tm merged_1_3_2) 2 vend_nothing vend"
-    apply (simp add: directly_subsumes_def)
-    apply (rule_tac x="[(''select'', [Str ''coke'']), (''coin'', [Num 50])]" in exI)
+  apply (simp add: directly_subsumes_def)
+  apply standard
+    apply (rule_tac x="[(STR ''select'', [Str ''coke'']), (STR ''coin'', [Num 50])]" in exI)
     apply standard
      apply (simp add: accepts_trace_def)
      apply (rule accepts.step)
@@ -838,7 +813,8 @@ proof-
     apply (simp add: merge_transitions_def easy_merge_def null_generator_def null_modifier_def)
     apply (simp add: no_direct_subsumption_vend_nothing_vend)
     apply (simp add: directly_subsumes_def)
-    apply (rule_tac x="[(''select'', [Str ''coke'']), (''coin'', [Num 50])]" in exI)
+    apply standard
+    apply (rule_tac x="[(STR ''select'', [Str ''coke'']), (STR ''coin'', [Num 50])]" in exI)
     apply standard
      apply (simp add: accepts_trace_def)
      apply (rule accepts.step)
@@ -929,7 +905,8 @@ proof-
     by eval
   have no_direct_subsumption_vend_nothing_vend: "\<not> directly_subsumes (tm DM_Inference.drinks2) (tm merged_4_5) 2 vend_nothing vend"
     apply (simp add: directly_subsumes_def)
-    apply (rule_tac x="[(''select'', [Str ''coke'']), (''coin'', [Num 50])]" in exI)
+    apply standard
+    apply (rule_tac x="[(STR ''select'', [Str ''coke'']), (STR ''coin'', [Num 50])]" in exI)
     apply standard
      apply (simp add: accepts_trace_def)
      apply (rule accepts.step)
@@ -948,7 +925,8 @@ proof-
     apply (simp add: merge_transitions_def easy_merge_def null_generator_def null_modifier_def leaves_5 leaves_4)
     apply (simp add: no_direct_subsumption_vend_nothing_vend)
     apply (simp add: directly_subsumes_def)
-    apply (rule_tac x="[(''select'', [Str ''coke'']), (''coin'', [Num 50])]" in exI)
+    apply standard
+    apply (rule_tac x="[(STR ''select'', [Str ''coke'']), (STR ''coin'', [Num 50])]" in exI)
     apply standard
      apply (simp add: accepts_trace_def)
      apply (rule accepts.step)
@@ -973,80 +951,17 @@ proof-
     by eval
   have leaves_4: "leaves 4 DM_Inference.drinks2 = 2"
     by eval
-  have no_direct_subsumption_vend_nothing_vend: "\<not> directly_subsumes (tm DM_Inference.drinks2) (tm merged_4_5) 2 vend_nothing vend"
-    apply (simp add: directly_subsumes_def)
-    apply (rule_tac x="[(''select'', [Str ''coke'']), (''coin'', [Num 50])]" in exI)
-    apply standard
-     apply (simp add: accepts_trace_def)
-     apply (rule accepts.step)
-      apply (simp add: step_def possible_steps_select_dm_2)
-     apply (rule accepts.step)
-      apply (simp add: step_def possible_steps_coin_dm_2)
-     apply (rule accepts.base)
-    apply standard
-    apply (rule gets_us_to.step_some)
-      apply (simp add: step_def possible_steps_select_dm_2)
-    apply (rule gets_us_to.step_some)
-      apply (simp add: step_def possible_steps_coin_dm_2)
-     apply (simp add: gets_us_to.base)
-  by (simp add: no_subsumption_vend_nothing_vend)
   show ?thesis
     apply (simp add: merge_transitions_def easy_merge_def null_generator_def null_modifier_def leaves_5 leaves_4)
-    apply (simp add: no_direct_subsumption_vend_nothing_vend)
-    apply (simp add: directly_subsumes_def)
-    apply (rule_tac x="[(''select'', [Str ''coke'']), (''coin'', [Num 50])]" in exI)
-    apply standard
-     apply (simp add: accepts_trace_def)
-     apply (rule accepts.step)
-      apply (simp add: step_def possible_steps_select_dm_2)
-     apply (rule accepts.step)
-      apply (simp add: step_def possible_steps_coin_dm_2)
-     apply (rule accepts.base)
-    apply standard
-    apply (rule gets_us_to.step_some)
-      apply (simp add: step_def possible_steps_select_dm_2)
-    apply (rule gets_us_to.step_some)
-      apply (simp add: step_def possible_steps_coin_dm_2)
-     apply (simp add: gets_us_to.base)
-    by (simp add: no_subsumption_vend_vend_nothing)
+    by (simp add: directly_subsumes_def no_subsumption_vend_vend_nothing no_subsumption_vend_nothing_vend)
 qed
 
 lemma cant_merge_vends_merged_1_3: "merge_transitions DM_Inference.drinks2 merged_1_3 2 1 1 1 1 vend 5 vend_nothing 1 null_generator null_modifier True = None"
-proof-
-  have no_direct_subsumption_vend_vend_nothing: "\<not> directly_subsumes (tm DM_Inference.drinks2) (tm merged_1_3) 1 vend vend_nothing"
-    apply (simp add: directly_subsumes_def accepts_trace_def)
-    apply (rule_tac x="[(''select'', [Str ''coke''])]" in exI)
-    apply standard
-     apply (rule accepts.step)
-      apply (simp add: step_def possible_steps_select_dm_2)
-     apply (simp add: accepts.base)
-    apply standard
-     apply (rule gets_us_to.step_some)
-      apply (simp add: possible_steps_select_dm_2 step_def)
-     apply (simp add: gets_us_to.base)
-    by (simp add: no_subsumption_vend_vend_nothing)
-  show ?thesis
-    apply (simp add: merge_transitions_def easy_merge_def null_generator_def null_modifier_def)
-    apply (simp add: no_direct_subsumption_vend_vend_nothing)
-    apply (simp add: directly_subsumes_def accepts_trace_def)
-    apply (rule_tac x="[(''select'', [Str ''coke'']), (''coin'', [Num 50])]" in exI)
-    apply standard
-     apply (rule accepts.step)
-      apply (simp add: step_def possible_steps_select_dm_2)
-     apply (rule accepts.step)
-      apply (simp add: step_def possible_steps_coin_dm_2)
-     apply (simp add: accepts.base)
-    apply standard
-     apply (rule gets_us_to.step_some)
-      apply (simp add: possible_steps_select_dm_2 step_def)
-     apply (rule gets_us_to.step_some)
-      apply (simp add: step_def possible_steps_coin_dm_2)
-     apply (simp add: gets_us_to.base)
-    by (simp add: no_subsumption_vend_nothing_vend)
-qed
+  apply (simp add: merge_transitions_def easy_merge_def null_generator_def null_modifier_def)
+  by (simp add: directly_subsumes_def no_subsumption_vend_vend_nothing no_subsumption_vend_nothing_vend)
 
-lemma gets_us_to_2_dm_2: "accepts_trace (tm DM_Inference.drinks2) [(''select'', [Str ''coke'']), (''coin'', [Num 50])] \<and>
-    gets_us_to 2 (tm DM_Inference.drinks2) 0 Map.empty [(''select'', [Str ''coke'']), (''coin'', [Num 50])]"
+lemma gets_us_to_2_dm_2: "accepts_trace (tm DM_Inference.drinks2) [(STR ''select'', [Str ''coke'']), (STR ''coin'', [Num 50])] \<and>
+    gets_us_to 2 (tm DM_Inference.drinks2) 0 Map.empty [(STR ''select'', [Str ''coke'']), (STR ''coin'', [Num 50])]"
   apply standard
   apply (simp add: accepts_trace_def)
      apply (rule accepts.step)
@@ -1060,8 +975,8 @@ lemma gets_us_to_2_dm_2: "accepts_trace (tm DM_Inference.drinks2) [(''select'', 
       apply (simp add: step_def possible_steps_coin_dm_2)
   by (simp add: gets_us_to.base)
 
-lemma gets_us_to_1_dm_2: "accepts_trace (tm DM_Inference.drinks2) [(''select'', [Str ''coke''])] \<and>
-    gets_us_to 1 (tm DM_Inference.drinks2) 0 Map.empty [(''select'', [Str ''coke''])]"
+lemma gets_us_to_1_dm_2: "accepts_trace (tm DM_Inference.drinks2) [(STR ''select'', [Str ''coke''])] \<and>
+    gets_us_to 1 (tm DM_Inference.drinks2) 0 Map.empty [(STR ''select'', [Str ''coke''])]"
   apply standard
   apply (simp add: accepts_trace_def)
      apply (rule accepts.step)
@@ -1074,34 +989,8 @@ lemma gets_us_to_1_dm_2: "accepts_trace (tm DM_Inference.drinks2) [(''select'', 
 lemma cant_merge_vends_merged_1_3_2: "merge_transitions DM_Inference.drinks2 (merge_states 1 3 merged_1_2) (leaves 1 DM_Inference.drinks2)
                      (leaves 5 DM_Inference.drinks2) (leaves 1 (merge_states 1 3 merged_1_2)) (arrives 1 (merge_states 1 3 merged_1_2))
                      (arrives 5 (merge_states 1 3 merged_1_2)) vend_nothing 1 vend 5 null_generator null_modifier True = None"
-proof-
-  have merge_1_3: "merge_states 1 3 merged_1_2 = {|
-    (0, (0, 1), select),
-    (1, (1, 1), vend_nothing),
-    (2, (1, 1), coin),
-    (3, (1, 1), coin),
-    (4, (1, 1), vend_fail),
-    (5, (1, 1), vend)
-  |}"
-    by eval
-  have leaves_5:  "leaves 5 DM_Inference.drinks2 = 2"
-    by eval
-  have leaves_1: "leaves 1 DM_Inference.drinks2 = 1"
-    by eval
-  have no_direct_subsumption_1: "\<not> directly_subsumes (tm DM_Inference.drinks2)
-        (tm {|(0, (0, 1), select), (1, (1, 1), vend_nothing), (2, (1, 1), coin), (3, (1, 1), coin), (4, (1, 1), vend_fail),
-              (5, (1, 1), vend)|})
-        (leaves 5 DM_Inference.drinks2) vend_nothing vend"
-    apply (simp add: directly_subsumes_def leaves_5)
-    apply (rule_tac x="[(''select'', [Str ''coke'']), (''coin'', [Num 50])]" in exI)
-    by (simp add: gets_us_to_2_dm_2 no_subsumption_vend_nothing_vend)
-  show ?thesis
-    apply (simp add: merge_1_3 Let_def merge_transitions_def easy_merge_def null_generator_def null_modifier_def)
-    apply (simp add: no_direct_subsumption_1)
-    apply (simp add: directly_subsumes_def leaves_1)
-    apply (rule_tac x="[(''select'', [Str ''coke''])]" in exI)
-    by (simp add: gets_us_to_1_dm_2 no_subsumption_vend_vend_nothing)
-qed
+  apply (simp add: merge_transitions_def easy_merge_def null_generator_def null_modifier_def)
+  by (simp add: directly_subsumes_def no_subsumption_vend_vend_nothing no_subsumption_vend_nothing_vend)
 
 lemma next_fmax: "fMax ({|(1::nat, (1::nat, 1::nat), (vend_fail, 4::nat), vend_nothing, 1::nat), (1, (1, 1), (coin, 3), coin, 2), (1, (1, 1), (coin, 2), coin, 3),
                         (1, (1, 3), (vend_nothing, 1), vend, 5), (1, (1, 1), (vend_nothing, 1), vend_fail, 4)|} |-|
@@ -1117,14 +1006,8 @@ lemma next_fmax_2: "fMax
 
 lemma cant_merge_vend_nothing_vend_2: "merge_transitions DM_Inference.drinks2 merged_1_3_2 2 2 (leaves 4 merged_1_3_2) (arrives 4 merged_1_3_2)
                      (arrives 5 merged_1_3_2) vend_nothing 4 vend 5 null_generator null_modifier True = None"
-proof-
-  show ?thesis
-    apply (simp add: merge_transitions_def easy_merge_def null_generator_def null_modifier_def)
-    apply (simp add: no_direct_subsumption_vend_nothing_vend)
-    apply (simp add: directly_subsumes_def)
-    apply (rule_tac x="[(''select'', [Str ''coke'']), (''coin'', [Num 50])]" in exI)
-    by (simp add: gets_us_to_2_dm_2 no_subsumption_vend_vend_nothing)
-qed
+  apply (simp add: merge_transitions_def easy_merge_def null_generator_def null_modifier_def)
+  by (simp add: directly_subsumes_def no_subsumption_vend_vend_nothing no_subsumption_vend_nothing_vend)
 
 lemma set_equiv_elem: "(s \<noteq> s') = (\<exists>e. (e \<in> s \<and> e \<notin> s') \<or> (e \<in> s' \<and> e \<notin> s))"
   by auto
@@ -1168,22 +1051,8 @@ lemma still_cant_merge_vends: "merge_transitions DM_Inference.drinks2
                                (arrives 5 (merge_states (arrives 5 merged_3_2_coins_2) (arrives 4 merged_3_2_coins_2) merged_3_2_coins_2))
                                (arrives 4 (merge_states (arrives 5 merged_3_2_coins_2) (arrives 4 merged_3_2_coins_2) merged_3_2_coins_2))
                                vend 5 vend_nothing 4 null_generator null_modifier True = None"
-proof-
-  have arrives_5: "arrives 5 merged_3_2_coins_2 = 3"
-    by eval
-  have arrives_4: "arrives 4 merged_3_2_coins_2 = 1"
-    by eval
-  have directly_subsumes_1: "\<not> directly_subsumes (tm DM_Inference.drinks2) (tm (merge_states 3 1 merged_3_2_coins_2)) 2 vend vend_nothing"
-    apply (simp add: directly_subsumes_def)
-    apply (rule_tac x="[(''select'', [Str ''coke'']), (''coin'', [Num 50])]" in exI)
-    by (simp add: gets_us_to_2_dm_2 no_subsumption_vend_vend_nothing)
-  show ?thesis
-    apply (simp add: merge_transitions_def easy_merge_def null_generator_def null_modifier_def)
-    apply (simp add: arrives_5 arrives_4 directly_subsumes_1)
-    apply (simp add: directly_subsumes_def)
-    apply (rule_tac x="[(''select'', [Str ''coke'']), (''coin'', [Num 50])]" in exI)
-    by (simp add: gets_us_to_2_dm_2 no_subsumption_vend_nothing_vend)
-qed
+  apply (simp add: merge_transitions_def easy_merge_def null_generator_def null_modifier_def)
+  by (simp add: directly_subsumes_def no_subsumption_vend_vend_nothing no_subsumption_vend_nothing_vend)
 
 lemma fminus_simp_2: "{|(1::nat, (1::nat, 1::nat), (coin, 2::nat), coin, 3::nat), (1, (1, 1), (coin, 3), coin, 2)|} |-| {|(1, (1, 1), (coin, 3), coin, 2)|} = {|(1, (1, 1), (coin, 2), coin, 3)|}"
   by eval
@@ -1194,25 +1063,8 @@ lemma stop_trying_to_merge_vends: "merge_transitions DM_Inference.drinks2
                                (arrives 4 (merge_states (arrives 4 merged_3_2_coins_2) (arrives 5 merged_3_2_coins_2) merged_3_2_coins_2))
                                (arrives 5 (merge_states (arrives 4 merged_3_2_coins_2) (arrives 5 merged_3_2_coins_2) merged_3_2_coins_2))
                                vend_nothing 4 vend 5 null_generator null_modifier True = None"
-proof-
-  have arrives_5: "arrives 5 merged_3_2_coins_2 = 3"
-    by eval
-  have arrives_4: "arrives 4 merged_3_2_coins_2 = 1"
-    by eval
-  have leaves_5: "leaves 5 DM_Inference.drinks2 = 2"
-    by eval
-  have directly_subsumes_1: "\<not> directly_subsumes (tm DM_Inference.drinks2) (tm (merge_states 1 3 merged_3_2_coins_2)) 2 vend_nothing
-        vend"
-    apply (simp add: directly_subsumes_def leaves_5)
-    apply (rule_tac x="[(''select'', [Str ''coke'']), (''coin'', [Num 50])]" in exI)
-    using gets_us_to_2_dm_2 no_subsumption_vend_nothing_vend by blast
-  show ?thesis
-    apply (simp add: merge_transitions_def easy_merge_def null_generator_def null_modifier_def)
-    apply (simp add: arrives_5 arrives_4 directly_subsumes_1)
-    apply (simp add: directly_subsumes_def leaves_5)
-    apply (rule_tac x="[(''select'', [Str ''coke'']), (''coin'', [Num 50])]" in exI)
-    using gets_us_to_2_dm_2 no_subsumption_vend_vend_nothing by blast
-qed
+  apply (simp add: merge_transitions_def easy_merge_def null_generator_def null_modifier_def)
+  by (simp add: directly_subsumes_def no_subsumption_vend_vend_nothing no_subsumption_vend_nothing_vend)
 
 lemma remove_max_nondetermnistic_pairs_merged_wrong_vends: "nondeterministic_pairs merged_wrong_vends |-| {|fMax (nondeterministic_pairs merged_wrong_vends)|} = {|(1, (1, 3), (vend_nothing, 4), vend, 5), (1, (1, 1), (coin, 2), coin, 3), (1, (1, 1), (coin, 3), coin, 2)|}"
   apply (simp add: nondeterministic_pairs_merged_wrong_vends max_def)
@@ -1326,19 +1178,8 @@ lemma no_vend_merge_1: "merge_transitions DM_Inference.drinks2 (merge_states (ar
            (arrives 5 (merge_states (arrives 5 merged_1_2) (arrives 1 merged_1_2) merged_1_2))
            (arrives 1 (merge_states (arrives 5 merged_1_2) (arrives 1 merged_1_2) merged_1_2)) vend 5 vend_nothing 1 null_generator
            null_modifier True = None"
-proof-
-  have directly_subsumes_1: "\<not> directly_subsumes (tm DM_Inference.drinks2) (tm (merge_states (arrives 5 merged_1_2) (arrives 1 merged_1_2) merged_1_2))
-        (leaves 1 DM_Inference.drinks2) vend vend_nothing"
-    apply (simp add: directly_subsumes_def leaves_1_dm2)
-    apply (rule_tac x="[(''select'', [Str ''coke''])]" in exI)
-    by (simp add: gets_us_to_1_dm_2 no_subsumption_vend_vend_nothing)
-  show ?thesis
-    apply (simp add: merge_transitions_def easy_merge_def null_generator_def null_modifier_def)
-    apply (simp add: directly_subsumes_1)
-    apply (simp add: directly_subsumes_def leaves_5_dm2)
-    apply (rule_tac x="[(''select'', [Str ''coke'']), (''coin'', [Num 50])]" in exI)
-    using gets_us_to_2_dm_2 no_subsumption_vend_nothing_vend by blast
-qed
+  apply (simp add: merge_transitions_def easy_merge_def null_generator_def null_modifier_def)
+  by (simp add: directly_subsumes_def no_subsumption_vend_vend_nothing no_subsumption_vend_nothing_vend)
 
 lemma no_vend_merge_2: "merge_transitions DM_Inference.drinks2 (merge_states (arrives 1 merged_1_2) (arrives 5 merged_1_2) merged_1_2)
            (leaves 1 DM_Inference.drinks2) (leaves 5 DM_Inference.drinks2)
@@ -1346,19 +1187,8 @@ lemma no_vend_merge_2: "merge_transitions DM_Inference.drinks2 (merge_states (ar
            (arrives 1 (merge_states (arrives 1 merged_1_2) (arrives 5 merged_1_2) merged_1_2))
            (arrives 5 (merge_states (arrives 1 merged_1_2) (arrives 5 merged_1_2) merged_1_2)) vend_nothing 1 vend 5 null_generator
            null_modifier True = None"
-proof-
-  have directly_subsumes_1: "\<not> directly_subsumes (tm DM_Inference.drinks2) (tm (merge_states (arrives 1 merged_1_2) (arrives 5 merged_1_2) merged_1_2))
-        (leaves 5 DM_Inference.drinks2) vend_nothing vend"
-    apply (simp add: directly_subsumes_def leaves_5_dm2)
-    apply (rule_tac x="[(''select'', [Str ''coke'']), (''coin'', [Num 50])]" in exI)
-    using gets_us_to_2_dm_2 no_subsumption_vend_nothing_vend by blast
-  show ?thesis
-    apply (simp add: merge_transitions_def easy_merge_def null_generator_def null_modifier_def)
-    apply (simp add: directly_subsumes_1 leaves_1_dm2)
-    apply (simp add: directly_subsumes_def)
-    apply (rule_tac x="[(''select'', [Str ''coke''])]" in exI)
-    by (simp add: gets_us_to_1_dm_2 no_subsumption_vend_vend_nothing)
-qed
+  apply (simp add: merge_transitions_def easy_merge_def null_generator_def null_modifier_def)
+  by (simp add: directly_subsumes_def no_subsumption_vend_vend_nothing no_subsumption_vend_nothing_vend)
 
 lemmas leaves_1_merged_1_2 = arrives_1_merged_1_2
 
